Liberation.thy
@@ -17,7 +17,7 @@ syntax
 translations
   "_liberate P x" == "CONST liberate P x"
 
-expr_ctr liberate
+expr_ctr liberate (0)
 
 lemma liberate_lens [expr_simps]: 
   "mwb_lens x \<Longrightarrow> P \\ $x = (\<lambda>s. \<exists>s'. P (s \<triangleleft>\<^bsub>x\<^esub> s'))"
